---
title: "Cox partial likelihood re-derived as normal equation of GLM"
subtitle: "Bypassing risk-set construction and event conditioning arguments"
date: "2025-02-16"
categories: [Biostatistics, Generalized Linear Models, Survival Analysis, Partial Likelihood]
format: html
image: images/cox_normal.png
open-graph: true
editor: visual
execute:
  eval: false
bibliography: references.bib
---

The Cox proportional hazards model is a popular *semiparametric* regression model in survival analysis. Its partial likelihood offers a clever way to filter out the nonparametric baseline function while keeping focus on the regression coefficients (log-hazard ratios).

The partial likelihood was originally derived through careful construction of risk sets and conditioning arguments specific to the survival context. However, with a bit of handwaving, I'll show that it can be re-derived, mechanically, as the "normal equation" of a generalized linear model (GLM).[^1]

## Normal equations of GLMs

Consider a GLM for response $Y$ against covariates $Z$: \begin{equation}\label{eq:mean_mod}
E(Y\mid Z) = \mu(\beta_0 + \beta^\mathrm{T} Z) \tag{1}
\end{equation} through some mean function $\mu(\cdot)$. The normal equation is defined as \begin{equation}\label{eq:normal}
\sum_{i=1}^n \left(\begin{array}{c}
1\\
Z_i\\
\end{array}\right)
\left\{Y_i - \mu(\beta_0 + \beta^\mathrm{T} Z_i)\right\} =0. \tag{2}
\end{equation} <!-- -   $\dot\mu(Z)=\d\mu(x)/\mathrm{d} x |_{x = \beta_0 + \beta^\mathrm{T} Z}$: differential of mean function;  --> <!-- -   $\sigma^2(Z) = {\rm var}(Y\mid Z)$: variance function. --> This is also the score equation for a GLM with a *canonical* link function. Solving \eqref{eq:normal} gives estimates of $\beta_0$ and $\beta$.

-   **Linear regression**: $\mu(x) = x$, with \eqref{eq:normal} leading to standard least squares.
-   **Logistic regression**: $\mu(x) = \exp(x)/\{1+\exp(x)\}$, with \eqref{eq:normal} corresponding to score equation for MLE.

## Cox model as a GLM

### Model specification

Let $T$ be the survival time of interest. The Cox model specifies \begin{equation}\label{eq:cox}
\lambda(t\mid Z) = \lambda_0(t)\exp(\beta^\mathrm{T} Z), \tag{3}
\end{equation} where $\lambda(t\mid Z)$ is the conditional hazard of $T$ given $Z$. However, this seems a bit far from the mean model formulation of \eqref{eq:mean_mod}.

### Reformulation as a mean model

Let's find a mean model implied by \eqref{eq:cox}. With censoring time $C$, we observe $X = \min(T, C)$ and $\delta = I(T\leq C)$. Write $N(t) = I(T\leq t, \delta = 1)$.

Consider $\mathrm{d} N(t)=N(t)-N(t-)$ as a binary response indicating an event observed at $t$. Then \eqref{eq:cox} implies \begin{align*}
E\{\mathrm{d} N(t)\mid X\geq t, Z\} &= I(X\geq t)\exp(\beta^\mathrm{T} Z)\lambda_0(t)\mathrm{d} t\\
&=I(X\geq t)\exp\{\beta_0(t)+\beta^\mathrm{T} Z\}.
\end{align*} where $\exp\{\beta_0(t)\}= \lambda_0(t)\mathrm{d} t$.

Now, we have a formulation similar to \eqref{eq:mean_mod} with $\mu(x) = I(X\geq t)\exp(x)$, though the intercept $\beta_0(t)$ is time-varying.

### Normal equation with time-varying intercept

Therefore, \eqref{eq:normal} becomes \begin{equation}\label{eq:normal_cox}
\sum_{i=1}^n\left(\begin{array}{c}
1\\
Z_i\\
\end{array}\right)
\big[\mathrm{d} N_i(t) - I(X_i\geq t)\exp\{\beta_0(t)+\beta^\mathrm{T} Z_i\}\big] =0.  \tag{4}
\end{equation}

Use the first-line equation in \eqref{eq:normal_cox} to solve for the "intercept" $$
\exp\{\hat\beta_0(t)\} = \frac{\sum_{i=1}^n \mathrm{d} N_i(t)}{\sum_{i=1}^n I(X_i\geq t)\exp(\beta^\mathrm{T} Z_i)}.
$$ Plugging it back to the left-hand side of \eqref{eq:normal_cox}:

\begin{align*}
&\sum_{i=1}^n Z_i\mathrm{d} N_i(t) - \exp\{\hat\beta_0(t)\}\sum_{i=1}^n  Z_iI(X_i\geq t)\exp(\beta^\mathrm{T} Z_i) \notag\\
=&\sum_{i=1}^n Z_i\mathrm{d} N_i(t) - \frac{\sum_{i=1}^n \mathrm{d} N_i(t)}{\sum_{i=1}^n I(X_i\geq t)\exp(\beta^\mathrm{T} Z_i)}\sum_{i=1}^n  Z_iI(X_i\geq t)\exp(\beta^\mathrm{T} Z_i) \notag\\
=& \sum_{i=1}^n \left\{Z_i - \frac{\sum_{j=1}^n  I(X_j\geq t)\exp(\beta^\mathrm{T} Z_j)Z_j}{\sum_{j=1}^n I(X_j\geq t)\exp(\beta^\mathrm{T} Z_j)}\right\}\mathrm{d} N_i(t) 
\end{align*} Integrating this over $t$ yields precisely the *partial-likelihood score* function.

## Conclusion

The Cox model can be reframed as a GLM for a binary event-indicator against an exponentially linked linear predictor with a time-dependent intercept. In this view, the partial likelihood score function aligns exactly with the normal equation of the GLM. This connection offers a new perspective on the Cox model and its estimation.

[^1]: **Whitehead (1980)** presented a similar derivation (Whitehead, J. “Fitting Cox’s Regression Model to Survival Data Using GLIM.” *Journal of the Royal Statistical Society Series C: Applied Statistics* 29 (3): 268. [https://doi.org/10.2307/2346901](https://doi.org/10.2307/2346901).)




